[Dafny] Make evaluate + correctness statement mutually recursive
To avoid unnecessary churn in regards to the correctness statement, we make
evaluate mutually recursive (like our compiler) by adding calls for expressions.

We also removed hard-coded values from the correctness statements.

compiler/dafny/semantics/dafny_evaluateScript.sml
@@ -9,7 +9,7 @@ open dafny_semanticPrimitivesTheory
 
 val _ = new_theory "dafny_evaluate";
 
-Type dafny_result = “:dafny_semanticPrimitives$result”
+Type dafny_result = “:'a dafny_semanticPrimitives$result”
 Type resultM = “:'a result_monad$result”
 Type program = “:module list”
 
@@ -201,15 +201,72 @@ Definition literal_to_value_def:
   literal_to_value _ = NONE
 End
 
-Definition evaluate_exp_def:
-  evaluate_exp (st: state) (env: sem_env)
-               (Literal l): (state # dafny_result) =
+(* Do an if-then-else *)
+(* TODO move to semantic primitives? *)
+Definition do_if_def:
+  do_if cnd thn els =
+    if cnd = BoolV T then SOME thn
+    else if cnd = BoolV F then SOME els
+    else NONE
+End
+
+(* Returns a list of names if none of the Formals has any attributes. *)
+Definition simple_formal_names_def:
+  simple_formal_names [] = SOME []
+  ∧
+  simple_formal_names ((Formal n _ [])::rest) =
+  (case (simple_formal_names rest) of
+   | SOME rest => SOME (n::rest)
+   | NONE => NONE)
+  ∧
+  simple_formal_names _ = NONE
+End
+
+Definition name_sig_call_def:
+  name_sig_call (Companion [mod_name] []) (CallName met_name NONE NONE F (CallSignature params inheritedParams)) =
+  SOME (dest_Ident mod_name, met_name, params, inheritedParams)
+  ∧
+  name_sig_call _ _ = NONE
+End
+
+Definition resolve_call_def:
+  resolve_call (env: sem_env) (exp_call: bool) (call_on: expression) (call_name: callName) call_typeArgs =
+  (case (name_sig_call call_on call_name) of
+   | NONE => INL Runsupported
+   | SOME (call_mod_name, call_met_name, call_params, call_inheritedParams) =>
+       (case (ALOOKUP env.methods (call_mod_name, call_met_name)) of
+        | NONE => INL Rtype_error
+        | SOME (Method met_attrs met_isStatic met_hasBody _ _
+                       met_overridingPath met_nam met_typeParams
+                       met_params met_inheritedParams met_body met_outTypes
+                       met_outVars) =>
+            (* Ignore outVarsAreUninitFieldsToAssign, wasFunction *)
+            if met_attrs ≠ [] ∨ ¬met_isStatic ∨ met_overridingPath ≠ NONE
+               ∨ met_typeParams ≠ [] ∨ call_typeArgs ≠ [] then
+              INL Runsupported
+            else if ¬met_hasBody ∨ met_nam ≠ call_met_name
+                    ∨ met_params ≠ call_params
+                    ∨ met_inheritedParams ≠ call_inheritedParams
+                    ∨ (exp_call ∧
+                       (LENGTH met_outTypes ≠ 1 ∨ met_outVars ≠ NONE)) then
+              INL Rtype_error
+            else
+              (* NOTE I believe that inheritedParams are mainly used in the Rust *)
+              (*   compiler to determine whether something needs to be borrowed. *)
+              (case (simple_formal_names met_params) of
+               | NONE => INL Runsupported
+               | SOME param_names => INR (param_names, met_body))))
+End
+
+(* Annotated with fix_clock *)
+Definition evaluate_stmts_ann_def[nocompute]:
+  evaluate_exp (st: state) (env: sem_env) (Literal l) : (state # value dafny_result) =
   (case literal_to_value l of
    | NONE => (st, Rerr Runsupported)  (* TODO Could also be Rtype_error *)
    | SOME v => (st, Rval v))
   ∧
   evaluate_exp st env (BinOp (TypedBinOp bop _ _ _) el er) =
-  (case evaluate_exp st env el of
+  (case fix_clock st (evaluate_exp st env el) of
    | (st', Rval vl) =>
        if is_lop bop then
          (case do_lop bop vl er of
@@ -223,36 +280,41 @@ Definition evaluate_exp_def:
                (* TODO Could also be Runsupported *)
                | NONE => (st'', Rerr Rtype_error)
                | SOME r => (st'', Rval r))
-           | r => r)
+          | r => r)
    | r => r)
   ∧
+  evaluate_exp st env (Expression_Call call_on call_name call_typeArgs call_args) =
+  (case (resolve_call env T call_on call_name call_typeArgs) of
+   | INL err => (st, Rerr err)
+   | INR (param_names, met_body) =>
+       (case fix_clock st (evaluate_exps st env call_args) of
+        | (st', Rval vals) =>
+            (case (push_param_frame st' param_names vals) of
+             | NONE => (st', Rerr Rtype_error)
+             | SOME st'' =>
+                 if st''.clock = 0
+                 then (st'', Rerr Rtimeout_error)
+                 else (evaluate_stmts (dec_clock st'') env met_body))
+        (* We mention this case explicitly to avoid type errors *)
+        | (st', Rerr err) => (st', Rerr err)))
+  ∧
   evaluate_exp st env _ = (st, Rerr Runsupported)
-Termination
-  WF_REL_TAC ‘measure $ expression_size o (λ(_,_,c). c)’ >> rw[]
-  >> gvs[do_lop_def, AllCaseEqs()]
-End
-
-Theorem evaluate_exp_clock:
-  ∀s1 env e r s2. evaluate_exp s1 env e = (s2, r) ⇒ s2.clock ≤ s1.clock
-Proof
-  ho_match_mp_tac evaluate_exp_ind >> rw[]
-  >> gvs[evaluate_exp_def, AllCaseEqs()]
-QED
-
-(* Do an if-then-else *)
-(* TODO move to semantic primitives? *)
-Definition do_if_def:
-  do_if cnd thn els =
-    if cnd = BoolV T then SOME thn
-    else if cnd = BoolV F then SOME els
-    else NONE
-End
-
-(* Annotated with fix_clock *)
-Definition evaluate_stmt_ann_def[nocompute]:
+  ∧
+  evaluate_exps st env [] : (state # (value list) dafny_result) =
+    (st, Rval [])
+  ∧
+  evaluate_exps st env (exp::exps) : (state # (value list) dafny_result) =
+  (case fix_clock st (evaluate_exp st env exp) of
+   | (st', Rval v) =>
+       (case (evaluate_exps st' env exps) of
+        | (sf, Rval vs) => (sf, Rval (v::vs))
+        | r => r)
+   (* We mention this case explicitly to avoid type errors *)
+   | (st', Rerr err) => (st', Rerr err))
+  ∧
   evaluate_stmt st env (DeclareVar varNam _ (SOME e) in_stmts) =
   (let varNam = dest_varName varNam in
-     (case evaluate_exp st env e of
+     (case fix_clock st (evaluate_exp st env e) of
       | (st', Rval v) =>
           (case add_local st' varNam v of
            | NONE => (st', Rerr Rtype_error)
@@ -264,7 +326,7 @@ Definition evaluate_stmt_ann_def[nocompute]:
      (case init_val t of
       | NONE => (st, Rerr Runsupported)
       | SOME v =>
-             (case add_local st varNam v of
+          (case add_local st varNam v of
               | NONE => (st, Rerr Rtype_error)
               | SOME st' => evaluate_stmts st' env in_stmts)))
   ∧
@@ -272,13 +334,13 @@ Definition evaluate_stmt_ann_def[nocompute]:
   (let varNam = dest_varName varNam in
      (case evaluate_exp st env e of
       | (st', Rval v) =>
-          (case assign_to_local st varNam v of
-           | NONE => (st, Rerr Rtype_error)
+          (case assign_to_local st' varNam v of
+           | NONE => (st', Rerr Rtype_error)
            | SOME st'' => (st'', Rval UnitV))
       | r => r))
   ∧
   evaluate_stmt st env (If cnd thn els) =
-  (case evaluate_exp st env cnd of
+  (case fix_clock st (evaluate_exp st env cnd) of
      (st', Rval v) =>
        (case do_if v thn els of
           NONE => (st', Rerr Rtype_error)
@@ -286,7 +348,7 @@ Definition evaluate_stmt_ann_def[nocompute]:
    | r => r)
   ∧
   evaluate_stmt st env (While e stmts) =
-  (case evaluate_exp st env e of
+  (case fix_clock st (evaluate_exp st env e) of
    | (st', Rval v) =>
        if v = BoolV F then (st', Rval UnitV)
        else if v = BoolV T then
@@ -301,60 +363,72 @@ Definition evaluate_stmt_ann_def[nocompute]:
          (st', Rerr Rtype_error)
    | r => r)
   ∧
-  evaluate_stmt (st: state) (env: sem_env) _ : (state # dafny_result) =
-    (st, Rerr Runsupported)
+  evaluate_stmt (st: state) (env: sem_env) _ =
+  (st, Rerr Runsupported)
   ∧
-  evaluate_stmts (st: state) (env: sem_env) [] : (state # dafny_result) =
-    (st, Rval UnitV)
+  evaluate_stmts (st: state) (env: sem_env) [] =
+  (st, Rval UnitV)
   ∧
-  evaluate_stmts (st: state) (env: sem_env)
-                 (stmt::stmts) : (state # dafny_result) =
-    (case fix_clock st (evaluate_stmt st env stmt) of
-     | (st', Rval _) =>
-         evaluate_stmts st' env stmts
-     | r => r)
+  evaluate_stmts (st: state) (env: sem_env) (stmt::stmts) =
+  (case fix_clock st (evaluate_stmt st env stmt) of
+   | (st', Rval _) =>
+       evaluate_stmts st' env stmts
+   | r => r)
 Termination
   WF_REL_TAC ‘inv_image ($< LEX $<)
               (λx. case x of
-                   | INL (s, _, stmt) =>
+                   | INL (s, _, exp) =>
+                       (s.clock, expression_size exp)
+                   | INR (INL (s, _, exps)) =>
+                       (s.clock, list_size expression_size exps)
+                   | INR (INR (INL (s, _, stmt))) =>
                        (s.clock, statement_size stmt)
-                   | INR (s, _, stmts) =>
-                       (s.clock, list_size statement_size stmts))’ >> rw[]
-  >> imp_res_tac evaluate_exp_clock
+                   | INR (INR (INR (s, _, stmts))) =>
+                       (s.clock, list_size statement_size stmts))’
+  >> rpt strip_tac
   >> imp_res_tac fix_clock_IMP
   >> gvs [dec_clock_def, AllCaseEqs(), assignLhs_size_eq, do_if_def,
-          add_local_def]
+          add_local_def, do_lop_def, push_param_frame_def]
 End
 
-Theorem evaluate_stmt_clock:
-  (∀s1 env stmt r s2.
-    evaluate_stmt s1 env stmt = (s2, r) ⇒ s2.clock ≤ s1.clock) ∧
-  (∀s1 env stmts r s2.
-    evaluate_stmts s1 env stmts = (s2, r) ⇒ s2.clock ≤ s1.clock)
+Theorem evaluate_stmts_clock:
+  (∀s₁ env exp r s₂.
+     evaluate_exp s₁ env exp = (s₂, r) ⇒ s₂.clock ≤ s₁.clock) ∧
+  (∀s₁ env exps r s₂.
+     evaluate_exps s₁ env exps = (s₂, r) ⇒ s₂.clock ≤ s₁.clock) ∧
+  (∀s₁ env stmt r s₂.
+     evaluate_stmt s₁ env stmt = (s₂, r) ⇒ s₂.clock ≤ s₁.clock) ∧
+  (∀s₁ env stmts r s₂.
+     evaluate_stmts s₁ env stmts = (s₂, r) ⇒ s₂.clock ≤ s₁.clock)
 Proof
-  ho_match_mp_tac evaluate_stmt_ann_ind >> rw[]
-  >> pop_assum mp_tac >> simp[Once evaluate_stmt_ann_def] >> strip_tac
-  >> gvs[AllCaseEqs(), dec_clock_def, fix_clock_def]
+  ho_match_mp_tac evaluate_stmts_ann_ind
+  >> rpt strip_tac
+  >> pop_assum mp_tac >> simp [Once evaluate_stmts_ann_def] >> strip_tac
+  >> gvs [AllCaseEqs (), dec_clock_def, fix_clock_def]
   >> EVERY (map imp_res_tac [add_local_clock, assign_to_local_clock,
-                             evaluate_exp_clock, fix_clock_IMP]) >> gvs[]
+                             push_param_frame_clock, fix_clock_IMP]) >> gvs[]
 QED
 
-Theorem fix_clock_evaluate_stmt:
-  fix_clock s1 (evaluate_stmt s1 env stmt) = evaluate_stmt s1 env stmt
+Theorem fix_clock_evaluate_stmts:
+  (fix_clock s₁ (evaluate_exp s₁ env exp) = evaluate_exp s₁ env exp) ∧
+  (fix_clock s₁ (evaluate_exps s₁ env exps) = evaluate_exps s₁ env exps) ∧
+  (fix_clock s₁ (evaluate_stmt s₁ env stmt) = evaluate_stmt s₁ env stmt) ∧
+  (fix_clock s₁ (evaluate_stmts s₁ env stmts) = evaluate_stmts s₁ env stmts)
 Proof
-  Cases_on ‘evaluate_stmt s1 env stmt’
-  \\ imp_res_tac evaluate_stmt_clock
-  \\ fs[fix_clock_def, state_component_equality]
+  Cases_on ‘evaluate_exp s₁ env exp’ >> Cases_on ‘evaluate_exps s₁ env exps’
+  >> Cases_on ‘evaluate_stmt s₁ env stmt’ >> Cases_on ‘evaluate_stmts s₁ env stmts’
+  >> imp_res_tac evaluate_stmts_clock
+  >> gvs [fix_clock_def, state_component_equality]
 QED
 
-Theorem evaluate_stmt_def[compute] =
-  REWRITE_RULE [fix_clock_evaluate_stmt] evaluate_stmt_ann_def;
+Theorem evaluate_stmts_def[compute] =
+  REWRITE_RULE [fix_clock_evaluate_stmts] evaluate_stmts_ann_def;
 
-Theorem evaluate_stmt_ind =
-  REWRITE_RULE [fix_clock_evaluate_stmt] evaluate_stmt_ann_ind;
+Theorem evaluate_stmts_ind =
+  REWRITE_RULE [fix_clock_evaluate_stmts] evaluate_stmts_ann_ind;
 
 Definition evaluate_def:
-  evaluate (p: program): (state # dafny_result) resultM =
+  evaluate (p: program): (state # value dafny_result) resultM =
   do
     env <- init_env p;
     main <- main_call env;
