compiler/dafny/semantics/dafny_compilerProofScript.sml
@@ -24,7 +24,7 @@ Type dafny_program = “:dafny_ast$module list”
 Type dafny_state = “:dafny_semanticPrimitives$state”
 Type dafny_env = “:dafny_semanticPrimitives$sem_env”
 Type dafny_exp = “:dafny_ast$expression”
-Type dafny_res = “:dafny_evaluate$dafny_result”
+Type dafny_res = “:'a dafny_evaluate$dafny_result”
 
 Type cakeml_program = “:ast$dec list”
 Type cakeml_state = “:simpleIO semanticPrimitives$state”
@@ -51,6 +51,7 @@ Definition dafny_to_cakeml_v_def[simp]:
   dafny_to_cakeml_v (StrV s) = (Litv (StrLit s))
 End
 
+(* TODO *)
 Definition state_rel_def:
   state_rel (s : dafny_state) (t : cakeml_state) ⇔ T
 End
@@ -60,7 +61,12 @@ Definition res_rel_def:
   res_rel (Rerr Rtype_error) (Rerr (Rabort Rtype_error)) = T ∧
   res_rel (Rerr Rtimeout_error) (Rerr (Rabort Rtimeout_error)) = T ∧
   res_rel (Rerr Runsupported) (_ : cakeml_res) = T ∧
-  res_rel (_ : dafny_res) (_ : cakeml_res) = F
+  res_rel (_ : value dafny_res) (_ : cakeml_res) = F
+End
+
+(* TODO *)
+Definition list_res_rel_def:
+  list_res_rel (r_dfy : (value list) dafny_res) (r_cml : cakeml_res) = T
 End
 
 Theorem res_rel_rval:
@@ -72,137 +78,52 @@ Proof
 QED
 
 Definition is_fail_dfy_def[simp]:
-  is_fail_dfy (Rerr _ : dafny_result) = T ∧
+  is_fail_dfy (Rerr _ : 'a dafny_result) = T ∧
   is_fail_dfy _ = F
 End
 
-Theorem correct_exp:
-  ∀ (s₁ : dafny_state) (env_dfy : dafny_env) (e : dafny_exp) (s₂ : dafny_state)
-    (r_dfy : dafny_res) (t₁ : cakeml_state) (env_cml : cakeml_env)
-    (cml_e : cakeml_exp).
-    evaluate_exp s₁ env_dfy e = (s₂, r_dfy) ∧ ¬(is_fail_dfy r_dfy) ∧
-    (* state_rel s₁ t₁ ∧ *) env_rel env_dfy env_cml ∧
-    from_expression (Companion [] []) e = INR cml_e ⇒
-    ∃ (t₂ : cakeml_state) (r_cml : cakeml_res).
-      evaluate$evaluate t₁ env_cml [cml_e] = (t₂, r_cml) ∧
-      (* state_rel s₂ t₂ ∧ *) res_rel r_dfy r_cml
-Proof
-  ho_match_mp_tac evaluate_exp_ind >> rw[]
-  >> pop_assum mp_tac >> simp [Once from_expression_def] >> strip_tac
-  >~ [‘BinOp’]
-  >- (gvs [evaluate_exp_def, CaseEq "prod",
-           CaseEq "dafny_semanticPrimitives$result"]
-      >- (Cases_on ‘bop’
-          >> gvs [is_lop_def, do_bop_def, AllCaseEqs ()]
-          >> (pop_assum mp_tac >> simp [Once from_expression_def] >> strip_tac
-              >> gvs[AllCaseEqs(), oneline bind_def])
-          >~ [‘Lt’]
-          >- (last_x_assum $ drule_then $ qspec_then ‘t₁’ strip_assume_tac
-              >> first_x_assum $ drule_then $ qspec_then ‘t₂’ strip_assume_tac
-              >> gvs [res_rel_rval, dafny_to_cakeml_v_def]
-              >> gvs [evaluate_def, do_app_def, opb_lookup_def])
-          >~ [‘Plus’]
-          >- (last_x_assum $ drule_then $ qspec_then ‘t₁’ strip_assume_tac
-              >> first_x_assum $ drule_then $ qspec_then ‘t₂’ strip_assume_tac
-              >> Cases_on ‘vl’ >> Cases_on ‘vr’
-              >> gvs [do_bop_def, dafny_to_cakeml_v_def, res_rel_rval]
-              >> gvs [evaluate_def, do_app_def, opn_lookup_def])
-          >~ [‘Minus’]
-          >- (last_x_assum $ drule_then $ qspec_then ‘t₁’ strip_assume_tac
-              >> first_x_assum $ drule_then $ qspec_then ‘t₂’ strip_assume_tac
-              >> Cases_on ‘vl’ >> Cases_on ‘vr’
-              >> gvs [do_bop_def, dafny_to_cakeml_v_def, res_rel_rval]
-              >> gvs [evaluate_def, do_app_def, opn_lookup_def])
-          >~ [‘Times’]
-          >- (last_x_assum $ drule_then $ qspec_then ‘t₁’ strip_assume_tac
-              >> first_x_assum $ drule_then $ qspec_then ‘t₂’ strip_assume_tac
-              >> Cases_on ‘vl’ >> Cases_on ‘vr’
-              >> gvs [do_bop_def, dafny_to_cakeml_v_def, res_rel_rval]
-              >> gvs [evaluate_def, do_app_def, opn_lookup_def])
-          >~ [‘And’]
-          >- (Cases_on ‘vl’ >> gvs [do_lop_def]
-              >> Cases_on ‘b’ >> gvs []
-              (* TODO Figure out why it is swapped here *)
-              >> first_x_assum $ drule_then $ qspec_then ‘t₁’ strip_assume_tac
-              >> last_x_assum $ drule_then $ qspec_then ‘t₂’ strip_assume_tac
-              >> gvs [res_rel_rval, dafny_to_cakeml_v_def]
-              >> gvs [evaluate_def, do_log_def])
-          >- (Cases_on ‘vl’ >> gvs [do_lop_def]
-              >> Cases_on ‘b’ >> gvs []
-              >> first_x_assum $ drule_then $ qspec_then ‘t₁’ strip_assume_tac
-              >> gvs [res_rel_rval, dafny_to_cakeml_v_def]
-              >> gvs [evaluate_def, do_log_def])
-          >- (Cases_on ‘vl’ >> gvs [do_lop_def]
-              >> Cases_on ‘b’ >> gvs []
-              (* TODO Figure out why it is swapped here *)
-              >> first_x_assum $ drule_then $ qspec_then ‘t₁’ strip_assume_tac
-              >> last_x_assum $ drule_then $ qspec_then ‘t₂’ strip_assume_tac
-              >> gvs [res_rel_rval, dafny_to_cakeml_v_def]
-              >> gvs [evaluate_def, do_log_def])
-          >- (Cases_on ‘vl’ >> gvs [do_lop_def]
-              >> Cases_on ‘b’ >> gvs []
-              >> first_x_assum $ drule_then $ qspec_then ‘t₁’ strip_assume_tac
-              >> gvs [res_rel_rval, dafny_to_cakeml_v_def]
-              >> gvs [evaluate_def, do_log_def])))
-  >~ [‘Literal’]
-  >- (Cases_on ‘l’ >> gvs [from_literal_def]
-      >~ [‘BoolLiteral’]
-      >- (Cases_on ‘b’ >> gvs [evaluate_exp_def, literal_to_value_def]
-          >> gvs [env_rel_def, evaluate_def, do_con_check_def, build_conv_def]
-          >> gvs [res_rel_def, dafny_to_cakeml_v_def,
-                  Boolv_def, bool_type_num_def])
-      >~ [‘IntLiteral’]
-      >- (gvs [AllCaseEqs (), oneline bind_def, string_to_int_def]
-          >> gvs [evaluate_exp_def, literal_to_value_def]
-          >> gvs [evaluate_def, res_rel_def, dafny_to_cakeml_v_def])
-      >~ [‘StringLiteral’]
-      >- gvs [evaluate_exp_def, literal_to_value_def]
-      >~ [‘Char’]
-      >- gvs [evaluate_exp_def, literal_to_value_def]
-      >~ [‘Null’]
-      >- gvs [evaluate_exp_def, literal_to_value_def])
-  >> gvs [evaluate_exp_def, literal_to_value_def]
-QED
-
 Theorem correct_stmts:
-  (∀ (s₁ : dafny_state) (env_dfy : dafny_env) (stmt : statement)
-     (s₂ : dafny_state) (r_dfy : dafny_res) (t₁ : cakeml_state)
-     (env_cml : cakeml_env) (cml_e : cakeml_exp).
-     evaluate_stmt s₁ env_dfy stmt = (s₂, r_dfy) ∧ ¬(is_fail_dfy r_dfy) ∧
-     state_rel s₁ t₁ ∧ env_rel env_dfy env_cml ∧
-     from_stmt (Companion [] []) 0 stmt Unit = INR cml_e
+  (∀ (s₁ : dafny_state) (env_dfy : dafny_env) (e : dafny_exp) (s₂ : dafny_state)
+     (r_dfy : value dafny_res) (t₁ : cakeml_state) (env_cml : cakeml_env)
+     (cml_e : cakeml_exp) (comp : expression).
+     evaluate_exp s₁ env_dfy e = (s₂, r_dfy) ∧
+     from_expression comp e = INR cml_e ∧ state_rel s₁ t₁ ∧
+     env_rel env_dfy env_cml ∧ ¬(is_fail_dfy r_dfy)
      ⇒ ∃ (t₂ : cakeml_state) (r_cml : cakeml_res).
          evaluate$evaluate t₁ env_cml [cml_e] = (t₂, r_cml) ∧
-         state_rel s₂ t₂ ∧ res_rel r_dfy r_cml)
-  ∧
+         state_rel s₂ t₂ ∧ res_rel r_dfy r_cml) ∧
+  (∀ (s₁ : dafny_state) (env_dfy : dafny_env) (es : dafny_exp list)
+     (s₂ : dafny_state) (r_dfy : (value list) dafny_res) (t₁ : cakeml_state)
+     (env_cml : cakeml_env) (cml_e : cakeml_exp) (comp : expression).
+     evaluate_exps s₁ env_dfy es = (s₂, r_dfy) ∧
+     map_from_expression comp es = INR cml_es ∧ state_rel s₁ t₁ ∧
+     env_rel env_dfy env_cml ∧ ¬(is_fail_dfy r_dfy)
+     ⇒ ∃ (t₂ : cakeml_state) (r_cml : cakeml_res).
+         evaluate$evaluate t₁ env_cml cml_es = (t₂, r_cml) ∧
+         state_rel s₂ t₂ ∧ list_res_rel r_dfy r_cml) ∧
+  (∀ (s₁ : dafny_state) (env_dfy : dafny_env) (stmt : statement)
+     (s₂ : dafny_state) (r_dfy : value dafny_res) (t₁ : cakeml_state)
+     (env_cml : cakeml_env) (cml_e : cakeml_exp) (comp : expression)
+     (lvl : int) (epi : exp).
+     evaluate_stmt s₁ env_dfy stmt = (s₂, r_dfy) ∧
+     from_stmt comp lvl stmt epi = INR cml_e ∧ state_rel s₁ t₁ ∧
+     env_rel env_dfy env_cml ∧ ¬(is_fail_dfy r_dfy)
+     ⇒ ∃ (t₂ : cakeml_state) (r_cml : cakeml_res).
+         evaluate$evaluate t₁ env_cml [cml_e] = (t₂, r_cml) ∧
+         state_rel s₂ t₂ ∧ res_rel r_dfy r_cml) ∧
   (∀ (s₁ : dafny_state) (env_dfy : dafny_env) (stmts : statement list)
-     (s₂ : dafny_state) (r_dfy : dafny_res) (t₁ : cakeml_state)
-     (env_cml : cakeml_env) (cml_e : cakeml_exp).
-     evaluate_stmts s₁ env_dfy stmts = (s₂, r_dfy) ∧ ¬(is_fail_dfy r_dfy) ∧
-     state_rel s₁ t₁ ∧ env_rel env_dfy env_cml ∧
-     from_stmts (Companion [] []) 0 stmts Unit = INR cml_e
+     (s₂ : dafny_state) (r_dfy : value dafny_res) (t₁ : cakeml_state)
+     (env_cml : cakeml_env) (cml_e : cakeml_exp) (comp : expression)
+     (lvl : int) (epi : exp).
+     evaluate_stmts s₁ env_dfy stmts = (s₂, r_dfy) ∧
+     from_stmts comp lvl stmts epi = INR cml_e ∧ state_rel s₁ t₁ ∧
+     env_rel env_dfy env_cml ∧ ¬(is_fail_dfy r_dfy)
      ⇒ ∃ (t₂ : cakeml_state) (r_cml : cakeml_res).
          evaluate$evaluate t₁ env_cml [cml_e] = (t₂, r_cml) ∧
          state_rel s₂ t₂ ∧ res_rel r_dfy r_cml)
 Proof
-  ho_match_mp_tac evaluate_stmt_ind >> rw[]
-  >> gvs [state_rel_def] (* This probably only works while it's defined as T *)
-  >~ [‘If’]
-  >- (gvs [Once from_expression_def, oneline bind_def, CaseEq "sum"]
-      >> gvs [evaluate_stmt_def, CaseEq "prod",
-              CaseEq "dafny_semanticPrimitives$result"]
-      >> gvs [do_if_def, CaseEq "option"]
-      >> Cases_on ‘v’ >> gvs []
-      >> Cases_on ‘b’ >> gvs []
-      (* from_expression cnd is properly compiled *)
-      >> drule correct_exp >> simp [] >> disch_then $ drule_at Any
-      >> disch_then $ qspec_then ‘t₁’ assume_tac >> gvs []
-      (* Apply induction hypothesis *)
-      >> first_x_assum $ qspec_then ‘t₂’ assume_tac
-      >> pop_assum $ drule_then assume_tac >> gs[]
-      (* Massage evaluate *)
-      >> gvs [res_rel_rval, evaluate_def,
-              semanticPrimitivesTheory.do_if_def])
+  ho_match_mp_tac evaluate_stmts_ind
+  >> rpt strip_tac
   >> cheat
 QED
 
